lts-v2, concat

LTS.thy
@@ -25,14 +25,16 @@ inductive LTS_is_reachable :: "('q, 'a) LTS  \<Rightarrow> 'q \<Rightarrow> 'a l
    LTS_Empty:"LTS_is_reachable \<Delta> q [] q"|
    LTS_Step:"(\<exists>q'' \<sigma>. a \<in> \<sigma> \<and> (q, \<sigma>, q'') \<in> \<Delta> \<and> LTS_is_reachable \<Delta> q'' w q') \<Longrightarrow> 
               LTS_is_reachable \<Delta> q (a # w) q'"|
-   LTS_Epi:"(\<exists>q''. (q,{},q'') \<in> \<Delta> \<and>  LTS_is_reachable \<Delta> q'' (a # w) q') \<Longrightarrow>   LTS_is_reachable \<Delta> q (a # w) q'"
+   LTS_Epi:"(\<exists>q''. (q,{},q'') \<in> \<Delta> \<and>  LTS_is_reachable \<Delta> q'' [] q') \<Longrightarrow>   LTS_is_reachable \<Delta> q [] q'"|
+   LTS_Epi1:"(\<exists>q''. (q,{},q'') \<in> \<Delta> \<and>  LTS_is_reachable \<Delta> q'' l q') \<Longrightarrow>   LTS_is_reachable \<Delta> q l q'"
 
 
 inductive_cases LTS_Step_cases:"LTS_is_reachable \<Delta> q (a # w) q'"
 
-inductive_cases LTS_Epi_cases:"LTS_is_reachable \<Delta> q l q'"
+inductive_cases LTS_Epi_cases:"LTS_is_reachable \<Delta> q [] q"
 
-inductive_cases LTS_Empty_cases:"LTS_is_reachable \<Delta> q [] q"
+inductive_cases LTS_Epi1_cases:"LTS_is_reachable \<Delta> q l q"
+
 
 
 lemma DeltLTSlemma1:"LTS_is_reachable Δ q al y \<Longrightarrow>LTS_is_reachable {(f u, v, f w)| u v w. (u,v,w)\<in> Δ } (f q) al (f y)"
@@ -40,14 +42,18 @@ proof (induction rule: LTS_is_reachable.induct)
   case (LTS_Empty Δ q)
   then show ?case 
     by (simp add: LTS_is_reachable.LTS_Empty)
-  next
+next
   case (LTS_Step a q Δ w q')
   then show ?case 
-    by (smt CollectI LTS_is_reachable.LTS_Step)
+    by (smt (verit, best) CollectI LTS_is_reachable.LTS_Step)
 next
-  case (LTS_Epi q Δ a w q')
-  then show ?case
-    by (smt LTS_is_reachable.LTS_Epi mem_Collect_eq)
+  case (LTS_Epi q Δ q')
+  then show ?case 
+    by (smt (verit, ccfv_threshold) CollectI LTS_is_reachable.LTS_Epi)
+next
+  case (LTS_Epi1 q Δ l q')
+  then show ?case 
+    by (metis (mono_tags, lifting) CollectI LTS_is_reachable.LTS_Epi1)
 qed
 
 
@@ -61,9 +67,13 @@ next
   then show ?case 
     by (meson LTS_is_reachable.LTS_Step UnI1)
 next
-  case (LTS_Epi q Δ a w q')
+  case (LTS_Epi q Δ q')
   then show ?case 
-    by (meson LTS_is_reachable.LTS_Epi UnCI)
+    by (meson LTS_is_reachable.LTS_Epi Un_iff)
+next
+  case (LTS_Epi1 q Δ l q')
+  then show ?case 
+    by (meson LTS_is_reachable.LTS_Epi1 UnI1)
 qed
 
 
